**Solutions.**

Three solutions are provided. The first employs induction,
the second one builds upon the first but adopts a linear algebra
perspective, and the final approach solves the problem 
combinatorically.

**Solution 1.**

At the beginning, it is important to illustrate the different patterns
under model JC69 with the following example when there are three species
($s = 3$). In total, the $4^{3} = 64$ combinations of nucleotides
collapse into the following five patterns denoted as
$aaa,\ abb,\ bab,\ bba,\ abc$.

111, where all three species have the same nucleotide:

* TTT, CCC, AAA, GGG

122, where the second and third species have the same nucleotide but the
first species has a different one.

* CTT, ATT, GTT, TCC, ACC, GCC, TAA, CAA, GAA, TGG, CGG, AGG

212, where the first and third species have the same nucleotide but the
* second species has a different one.

221, where the first and second species have the same nucleotide but the
* third species has a different one.

123, where all three species have different nucleotides.
* TCG, GCT, GAT, GTA, CTG, ACG, ACT, CGT, GTC, TGC, GAC, CGA, GCA, TGA,
AGC, TAC, ATG, ATC, CTA, TCA, AGT, CAT, TAG, CAG

Now, denfine $f(s) = \frac{4^{s - 1} + 3 \times 2^{s - 1} + 2}{6}$, the
formula given in the problem. Denote $E_{s}$ as the set of the different
patterns for $s$ species, $A_{s}$ as the set where each element consists
of only a single state, $B_{s}$ as the set where each element consists
of exactly two states, $C_{s}$ as the set where each element consists of
three states, and $D_{s}$ as the set where each element consists of
three states. It is easy to see that $A_{s},B_{s},C_{s},D_{s}$ are
disjoint sets. Equivalently,

$$E_{s} = A_{s} \cup B_{s} \cup C_{s} \cup D_{s},\ with\ A_{s} \cap B_{s} = A_{s} \cap C_{s} = \ldots = C_{s} \cap D_{s} = \varnothing.$$

In the above example,
$A_{3}=$ $`\{111\}`$, $B_{3} =$ $`\{122,212,221\}`$, $C_{3} =$ $`\{123\}`$.

1\) It is easy to verify that the given formula holds for $s = 1,\ 2$.

2\) When $s = 3$, there are the following five patterns $aaa$ (all the
same), $baa,\ aba,\ aab$ (one different from the others), and $abc$ (all
different), satisfying
$f(3) = \frac{4^{3 - 1} + 3 \times 2^{3 - 1} + 2}{6} = 5$.

3\) When $s = 4$, there are 15 patterns (see below), well meeting the
given formula
$f(4) = \frac{4^{4 - 1} + 3 \times 2^{4 - 1} + 2}{6} = 15$. Further
divide the 15 patterns into three disjoint sets according to the number
of states that each element has as follows

$$E_{4} = A_{4} \cup B_{4} \cup C_{4} \cup D_{4},$$

where $A_{4} = \{ 1111\}$,
$B_{4} = \{ 1111,\ 1121,\ 1211,\ 2111,\ 1122,\ 1212,\ 1221\}$,
$C_{4} = \{ 1123,\ 1213,\ 1231,\ 2311,\ 2131,\ 2113\}$,
$D_{4} = \{ 1234\}$. We also have the numbers of elements in the above
sets
$\left| A_{4} \right| = 1,\ \left| B_{4} \right| = 7,\ \left| C_{4} \right| = 7$.

4\) As to $s = 5$, we have the following result based on the above
pattern for $s = 4$.

Divide the set $E_{5}$ into four disjoint sets according to the number
of states of its elements as follows

$$
\begin{align*}
A_{5} &= \{11111\}, \\
B_{5} &= \{2\} \times A_{4} \cup \{1,2\} \times B_{4}, \\
C_{5} &= \{3\} \times B_{4} \cup \{1,2,3\} \times C_{4}, \\
D_{5} &= \{4\} \times C_{4} \cup \{1,2,3,4\} \times D_{4}.
\end{align*}
$$

and apparently we have

$$
\begin{align*}
\left| A_{5} \right| &= |A_{4}| = 1, \\
\left| B_{5} \right| &= 1 + 2 \times |B_{4}| = 15, \\
\left| C_{5} \right| &= 1 \times |B_{4}| + 3 \times |C_{4}| = 28, \\
\left| D_{5} \right| &= 1 \times \left| C_{4} \right| + 4 \times \left| D_{4} \right| = 7.
\end{align*}
$$

So

$${|E}_{5}| = 1 + 15 + 28 + 7 = 51 = \frac{4^{5 - 1} + 3 \times 2^{5 - 1} + 2}{6} = f(5).$$

5\) As to $s = 6$, likewise, we can have the following result based on
the above patterns for $s = 5$. $
$Again, divide set $E_{5}$ into three disjoint sets according to the
number of states of the elements as follows

$$
\begin{align*}
A_{6} &= \{ 111111 \}, \\
B_{6} &= ( \{ 2 \} \times A_{5} ) \cup ( \{ 1,2 \} \times B_{5} ), \\
C_{6} &= ( \{ 3 \} \times B_{5} ) \cup (\{ 1,2,3 \} \times C_{5}), \\
D_{6} &= ( \{ 4 \} \times C_{5} ) \cup ( \{ 1,2,3,4 \} \times D_{5} ).
\end{align*}
$$


and we have
$\left| A_{6} \right| = 1$,
$\left| B_{6} \right| = 1 + 2 \times |B_{5}| = 31$,
$\left| C_{6} \right| = 1 \times \left| B_{5} \right| + 3 \times \left| C_{5} \right| = 99,\left| D_{6} \right| = 1 \times \left| C_{5} \right| + 4 \times \left| D_{5} \right| = 56$.

So

$${|E}_{6}| = 1 + 31 + 99 + 56 = 187 = \frac{4^{6 - 1} + 3 \times 2^{6 - 1} + 2}{6} = f(6).$$

You of course can do similar stuff for $s = 7,8,\ldots$, but at this
point, it may be clear enough to see the following

$$
\begin{align*}
A_{s} &= \{ 1 \} \times \{ A_{s - 1} \}, \\
B_{s} &= ( \{ 2 \} \times A_{s - 1} ) \cup ( \{ 1,2 \} \times B_{s - 1} ), \\
C_{s} &= ( \{ 3 \} \times B_{s - 1} ) \cup ( \{ 1,2,3 \} \times C_{s - 1} ), \\
D_{s} &= ( \{ 4 \} \times C_{s - 1} ) \cup ( \{ 1,2,3,4 \} \times D_{s - 1} ).
\end{align*} \tag{4.1}
$$


Hence, the total number of patterns for any given $s$ can be calculated as

$$
\begin{align*}
f(s) = \left| E_{s} \right| 
&= \left| A_{s} \right| + \left| B_{s} \right| + \left| C_{s} \right| + \left| D_{s} \right| \\
&= \left| A_{s - 1} \right| \times 1 + \left( 1 + \left| B_{s - 1} \right| \times 2 \right) + \left( \left| B_{s - 1} \right| + \left| C_{s - 1} \right| \times 3 \right) + \left( \left| C_{s - 1} \right| + \left| D_{s - 1} \right| \times 4 \right) \\
&= \left| A_{s - 1} \right| + \left| B_{s - 1} \right| \times 3 + \left( \left| C_{s - 1} \right| + |D_{s - 1}| \right) \times 4
\end{align*}
$$

where $\left| A_{s} \right| \equiv 1$ for any $s$.

As follows we apply induction. It is obvious from the above
that $f(s)$ holds for $s = 1,2,3,4$. Suppose
$f(s) = \frac{4^{s - 1} + 3 \times 2^{s - 1} + 2}{6}$ holds for all
values up to some $k$. Compare $f(k + 1)$ and $f(k)$, and by eliminating
the items containing $|C_{k - 1}|$ or $|D_{k - 1}|$, we can further show
that

$$
\begin{align*}
f(k + 1) &= 4 \times \left( |A_{k - 1}| + \left| B_{k - 1} \right| + \left| C_{k - 1} \right| + \left| D_{k - 1} \right| \right) - \left( \left| B_{k - 1} \right| \times 2 + 3 \right) \\
&= 4f(k) - \left( 2\left| B_{k - 1} \right| + 3 \right).
\end{align*}
$$

Now our focus shifts to $|B_{k}|$.The elements of $|B_{k}|$ consist of
two sources. One is $\{\underset{k\ times}{\overset{aa\ldots a}{ï¸¸}}\}$,
which is a singleton set. The other is composed of those with exactly
two states from $B_{k - 1}$. Consider a few different values for $s$:

$$
{\left| B_{4} \right| = 7 \times 1
}{\left| B_{5} \right| = 1 + 7 \times 2
}{\left| B_{6} \right| = 1 + (1 + 7 \times 2) \times 2
}{\left| B_{7} \right| = 1 + 2 \times \left( 1 + 2 \times (1 + 7 \times 2) \right).}
$$

It is not difficult to see the following

$$\left| B_{k} \right| = 2^{k - 4} \times 7\  + \ 2^{k - 4} - 1,$$

thus

$$\left| B_{k - 1} \right| = 2^{k - 5} \times 7 + 2^{k - 5} - 1,$$

where $s \geq 4$. Introducing the expression of $\left| B_{k - 1} \right|$ to $f(k + 1)$, we have

$$
\begin{align*}
f(k + 1) &= \frac{4^{k - 1} + 3 \times 2^{k - 1} + 2}{6} - 2 \times (2^{k - 5} \times 7 + 2^{k - 5} - 1) - 3 \\
&= \frac{2 \times 4^{k - 1} + (6 \times 2^{k - 1} - 48 \times 2^{k - 5} + 1)}{3} \\
&= \frac{4^{k} + 6 \times 2^{k} - 3 \times 2^{5} \times 2^{k - 5} + 2}{6}\ (both\ top\ and\ bottom \times 2) \\
&= \frac{4^{k} + 3 \times 2^{k} + 2}{6}
\end{align*}
$$

**Solution 2.**

Define
$a_{s} = \left| A_{s} \right|,\ b_{s} = \left| B_{s} \right|,\ c_{s} = \left| C_{s} \right|,\ d_{s} = \left| D_{s} \right|,\ e_{s} = |E_{s}|$.

Starting from Eq. (4.1), we can re-write it in the form of matrix as

$$\begin{bmatrix}
a_{s + 1} \\
b_{s + 1} \\
c_{s + 1} \\
d_{s + 1} \\
\end{bmatrix} = \begin{bmatrix}
1 & 0 & 0 & 0 \\
1 & 2 & 0 & 0 \\
0 & 1 & 3 & 0 \\
0 & 0 & 1 & 4 \\
\end{bmatrix}\begin{bmatrix}
a_{s} \\
b_{s} \\
c_{s} \\
d_{s} \\
\end{bmatrix}.$$

Further define

$$W = \begin{bmatrix}
1 & 0 & 0 & 0 \\
1 & 2 & 0 & 0 \\
0 & 1 & 3 & 0 \\
0 & 0 & 1 & 4 \\
\end{bmatrix}.$$

Apparently,

$$\left( a_{1},b_{1},c_{1},d_{1} \right)^{T} = (1,0,0,0)^{T}.$$

It follows that

$$\begin{bmatrix}
a_{s + 1} \\
b_{s + 1} \\
c_{s + 1} \\
d_{s + 1} \\
\end{bmatrix} = W\begin{bmatrix}
a_{s} \\
b_{s} \\
c_{s} \\
d_{s} \\
\end{bmatrix} = W^{2}\begin{bmatrix}
a_{s - 1} \\
b_{s - 1} \\
c_{s - 1} \\
d_{s - 1} \\
\end{bmatrix} = \ldots = W^{s}\begin{bmatrix}
1 \\
0 \\
0 \\
0 \\
\end{bmatrix}.$$

We can do Eigenvalue decomposition for $W$ as follows

$$W = P\Lambda P^{- 1}$$

where

$$
\Lambda = \text{diag}(1,2,3,4),
$$

$$
P = \begin{bmatrix}
-6 & 0 & 0 & 0 \\
6 & 2 & 0 & 0 \\
-3 & -2 & -1 & 0 \\
1 & 1 & 1 & 1 \\
\end{bmatrix},
$$

$$
P^{-1} = \begin{bmatrix}
-1/6 & 0 & 0 & 0 \\
1/2 & 1/2 & 0 & 0 \\
-1/2 & -1 & -1 & 0 \\
1/6 & 1/2 & 1 & 1 \\
\end{bmatrix}.
$$

Hence,

$$
\begin{align*}
\begin{bmatrix}
a_{s + 1} \\
b_{s + 1} \\
c_{s + 1} \\
d_{s + 1} \\
\end{bmatrix} &= P\Lambda^{s}P^{-1}\begin{bmatrix}
1 \\
0 \\
0 \\
0 \\
\end{bmatrix} \\
&= \begin{bmatrix}
-6 & 0 & 0 & 0 \\
6 & 2 & 0 & 0 \\
-3 & -2 & -1 & 0 \\
1 & 1 & 1 & 1 \\
\end{bmatrix}\begin{bmatrix}
1 & 0 & 0 & 0 \\
0 & 2^{s} & 0 & 0 \\
0 & 0 & 3^{s} & 0 \\
0 & 0 & 0 & 4^{s} \\
\end{bmatrix}\begin{bmatrix}
-1/6 & 0 & 0 & 0 \\
1/2 & 1/2 & 0 & 0 \\
-1/2 & -1 & -1 & 0 \\
1/6 & 1/2 & 1 & 1 \\
\end{bmatrix}\begin{bmatrix}
1 \\
0 \\
0 \\
0 \\
\end{bmatrix} \\
&= \begin{bmatrix}
-6 & 0 & 0 & 0 \\
6 & 2 & 0 & 0 \\
-3 & -2 & -1 & 0 \\
1 & 1 & 1 & 1 \\
\end{bmatrix}\begin{bmatrix}
-1/6 & 0 & 0 & 0 \\
2^{s - 1} & 2^{s} & 0 & 0 \\
-3^{s}/2 & 0 & 3^{s} & 0 \\
4^{s}/6 & 2^{s - 1} & -3^{s}/2 & 3^{s} \\
\end{bmatrix} \\
&= \begin{bmatrix}
1 \\
2^{s} - 1 \\
1/2 - 2^{s} + 3^{s}/2 \\
2^{s - 1} - 3^{s}/2 + 4^{s}/6 - 1/6 \\
\end{bmatrix}.
\end{align*}
$$

Thus

$$
\begin{align*}
f(s + 1) &= 1 + (2^{s} - 1) + (1/2 - 2^{s} + 3^{s}/2) + (2^{s - 1} - 3^{s}/2 + 4^{s}/6 - 1/6) \\
&= (4^{s} + 3 \times 2^{s} + 2)/6.
\end{align*}
$$

So

$$
f(s) = (4^{s - 1} + 3 \times 2^{s - 1} + 2)/6.
$$


**Solution 3.**

This solution uses a combinatorics way. Let $X$ denote the set of all
sequences composed of $n$ types of nucleotides. Let $Y_{i}$ denote the
set of sequences where the $i$-th type of nucleotide does not appear.
Let $Z$ denote the set of sequences where all $m$ types of nucleotides
appear. Let us take an example. For cases where $m = 3$ and $n = 3$, we
have

$$
X = \\{ 111,112,113,\ldots,333 \\},
$$

$$
Y_{1} = \\{ 222,223,232,\ldots,333 \\},
$$

$$
Y_{2} = \\{ 111,113,131,\ldots,333 \\},
$$

$$
Y_{3} = \\{ 111,112,121,\ldots,222 \\},
$$

$$
Z = \\{ 123,132,213,231,312,321 \\},
$$


where $1,2,3$ denote the different states (note again that in this
example $m = 3$). It is easy to see

$$|X| = 27,\left| Y_{1} \right| = \left| Y_{2} \right| = \left| Y_{3} \right| = 8,|Z| = 6.$$

In general, we have

$$
\begin{align*}
|X| &= m^{n}, \\
|Z| &= |X| - |Y_{1} \cup Y_{2} \cup \ldots \cup Y_{m}|, \\
|Y_{1} &= |Y_{2}| = \ldots = |Y_{m}| = (m - 1)^{n}, \\
|Y_{1} \cap Y_{2}| &= |Y_{1} \cap Y_{3}| = \ldots = |Y_{m - 1} \cap Y_{m}| = (m - 2)^{n}, \\
|Y_{1} \cap Y_{2} \cap Y_{3}| &= |Y_{1} \cap Y_{2} \cap Y_{4}| = \ldots = |Y_{m - 2} \cap Y_{m-1} \cap Y_{m}| = (m - 3)^{n}, \\
&\vdots \\
|Y_{1} \cap Y_{2} \cap \ldots \cap Y_{m}| &= (m - m)^{n} = 0.
\end{align*}
$$

Apply the inclusion-exclusion principle. It follows that

$$
\begin{align*}
\left| Y_{1} \cup Y_{2} \cup \ldots \cup Y_{m} \right| &= \sum_{i = 1}^{m}\left| Y_{i} \right| - \sum_{i = 1}^{m - 1}{\sum_{j = i + 1}^{m}\left| Y_{i} \cap Y_{j} \right|} + \sum_{i = 1}^{m - 2}{\sum_{j = i + 1}^{m - 1}{\sum_{k = j + 1}^{m}\left| Y_{i} \cap Y_{j} \cap Y_{k} \right|}} + \ldots + ( - 1)^{m}\left| Y_{1} \cap Y_{2} \cap \ldots \cap Y_{m} \right| \\
&= \begin{pmatrix}
m \\
1 \\
\end{pmatrix}(m - 1)^{n} + ( - 1)^{1}\begin{pmatrix}
m \\
2 \\
\end{pmatrix}(m - 2)^{n} + ( - 1)^{2}\begin{pmatrix}
m \\
3 \\
\end{pmatrix}(m - 3)^{n} + \ldots + ( - 1)^{m - 1}\begin{pmatrix}
m \\
m \\
\end{pmatrix}(m - m)^{n} \\
&= \sum_{k = 1}^{m}{( - 1)^{k - 1}\begin{pmatrix}
m \\
k \\
\end{pmatrix}(m - k)}^{n}.
\end{align*}
$$

Therefore, we have

$$
\begin{align*}
|Z| &= |X| - \left| Y_{1} \cup Y_{2} \cup \ldots \cup Y_{m} \right| \\
&= m^{n} - \sum_{k = 1}^{m}{( - 1)^{k - 1}\begin{pmatrix}
m \\
k \\
\end{pmatrix}(m - k)}^{n} \\
&= {{- ( - 1)}^{0 - 1}\begin{pmatrix}
m \\
0 \\
\end{pmatrix}(m - 0)}^{n} - \sum_{k = 1}^{m}{( - 1)^{k - 1}\begin{pmatrix}
m \\
k \\
\end{pmatrix}(m - k)}^{n} \\
&= - 1 \times \left( \sum_{k = 0}^{m}{( - 1)^{k - 1}\begin{pmatrix}
m \\
k \\
\end{pmatrix}(m - k)}^{n} \right) \\
&= \sum_{k = 0}^{m}{( - 1)^{k}\begin{pmatrix}
m \\
k \\
\end{pmatrix}(m - k)}^{n}.
\end{align*}
$$

Now, denote in a sequence of length $n$ there are $a_{m,n}$ combinations
that have exactly $m$ states (types of nucleotides). Equivalently,

$$a_{m,n} = \sum_{k = 0}^{m}{( - 1)^{k}\begin{pmatrix}
m \\
k \\
\end{pmatrix}(m - k)}^{n}.$$

Denote $b_{m,n}$ as the number of patterns with given $m$ and $n$. Note
that $b_{m,n}$ differs from $a_{m,n}$ in that it refers to the number of
patterns instead of combinations. As an example, the combination "TTT"
and "CCC" refer to the same pattern which can be denoted by "111".
Hence,

$$b_{m,n} = \frac{a_{m,n}}{m!}.$$

According to the context, the number of patterns for four types of
nucleotides thus $m = 1,2,3,4$ may be calculated as

$$\sum_{m = 1}^{4}b_{m,n} = \sum_{m = 1}^{4}\frac{a_{m,n}}{m!}.$$

Hence

$$
a_{1,1} = {\begin{pmatrix}
1 \\
0 \\
\end{pmatrix}(1 - 0)}^{n} = 1,
$$

$$
{{a_{2,1} = \begin{pmatrix}
2 \\
0 \\
\end{pmatrix}(2 - 0)}^{n} - {\begin{pmatrix}
2 \\
1 \\
\end{pmatrix}(2 - 1)}^{n} = 2^{n} - 2,
}
$$

$$
{a_{3,1} = {\begin{pmatrix}
3 \\
0 \\
\end{pmatrix}(3 - 0)}^{n} - {\begin{pmatrix}
3 \\
1 \\
\end{pmatrix}(3 - 1)}^{n} + {\begin{pmatrix}
3 \\
2 \\
\end{pmatrix}(3 - 2)}^{n} = 3^{n} - 3 \times 2^{n} + 3,
}
$$

$$
{a_{4,1} = {\begin{pmatrix}
4 \\
0 \\
\end{pmatrix}(4 - 0)}^{n} - {\begin{pmatrix}
4 \\
1 \\
\end{pmatrix}(4 - 1)}^{n} + {\begin{pmatrix}
4 \\
2 \\
\end{pmatrix}(4 - 2)}^{n} - {\begin{pmatrix}
4 \\
3 \\
\end{pmatrix}(4 - 3)}^{n} = 4^{n} - 4 \times 3^{n} + 6 \times 2^{n} - 4.}
$$

Therefore, the total number of patterns can be calculated as

$$
\begin{align*}
\sum_{m = 1}^{4}\frac{a_{m,n}}{m!} &= \frac{1}{1!} + \frac{2^{n} - 2}{2!} + \frac{3^{n} - 3 \times 2^{n} + 3}{3!} + \frac{4^{n} - 4 \times 3^{n} + 6 \times 2^{n} - 4}{4!} \\
&= 1 + 2^{n - 1} - 1 + \frac{3^{n} - 3 \times 2^{n} + 3}{6} + \frac{4^{n - 1} - 3^{n} + 3 \times 2^{n - 1} - 1}{6} \\
&= \frac{3 \times 2^{n} + 3^{n} - 3 \times 2^{n} + 3 + 4^{n - 1} - 3^{n} + 3 \times 2^{n - 1} - 1}{6} \\
&= \frac{4^{n - 1} + 3 \times 2^{n - 1} + 2}{6}.
\end{align*}
$$

