**Solution.**

a\) According to the context, $A$ denotes the event that a person is
infected, and $B$ denotes the event that a person tests positive.
According to the Bayes' theorem, it follows that

$$
\begin{align*}
P\left( A|\overline{B} \right) &= \frac{P(A)P\left( \overline{B} \middle| A \right)}{P\left( \overline{B} \right)} \\
&= \frac{P(A)\left( 1 - P\left( B \middle| A \right) \right)}{1 - P(B)} \\
&= \frac{P(A)\left( 1 - P\left( B \middle| A \right) \right)}{1 - \left( P(A)P\left( B \middle| A \right) + \left( 1 - P(A) \right)P\left( B \middle| \overline{A} \right) \right)}.
\end{align*}
$$

Introducing $P\left( B \middle| A \right) = 0.99$,
$P\left( B \middle| \overline{A} \right) = 0.02$, $P(A) = 0.001$ as
given in Section 5.1.2 of (Yang, 2006), we have

$$\begin{align*}
P\left( A|\overline{B} \right) &= \frac{0.001 \times (1 - 0.99)}{1 - (0.001 \times 0.99 - 0.999 \times 0.02)} \\
&= 1.021419e - 05.
\end{align*}
$$

b\) Denote $C$ as the event that a person tests positive twice. It
follows that

$$
\begin{align*}
P\left( A \middle| C \right) &= \frac{P(A)P\left( C \middle| A \right)}{P(C)} \\
&= \frac{P(A)P\left( B \middle| A \right)P\left( B \middle| A \right)}{P(A)P\left( C|A \right) + P\left( \overline{A} \right)P\left( C|\overline{A} \right)} \\
&= \frac{P(A)P\left( B \middle| A \right)P\left( B \middle| A \right)}{P(A)P\left( B|A \right)P\left( B|A \right) + P\left( \overline{A} \right)P\left( B|\overline{A} \right)P\left( B|\overline{A} \right)} \\
&= \frac{0.001 \times {0.99}^{2}}{0.001 \times {0.99}^{2} + 0.999 \times {0.02}^{2}} \\
&= 0.7103718.
\end{align*}
$$
