**Solution.**

First, calculate the eigenvalues and eigenvectors of *Q*.

$$
\begin{align*}
\left| \begin{matrix}
-u - \lambda & u \\
v & -v - \lambda \\
\end{matrix} \right| &= 0
\end{align*}
$$

By solving the following equation

$$
\begin{align*}
\lambda^{2} + (u + v)\lambda &= 0
\end{align*}
$$

we get the eigenvalues and their corresponding eigenvectors:

$$
\begin{align*}
\lambda_{1} &= 0, \quad \lambda_{2} = -u - v, \\
v_{1} &= \begin{bmatrix}
1 \\
1 \\
\end{bmatrix}, \quad v_{2} = \begin{bmatrix}
-u \\
v \\
\end{bmatrix}.
\end{align*}
$$

Hence,

$$
\begin{align*}
P(t) &= e^{Qt} \\
&= \begin{bmatrix}
1 & -u \\
1 & v \\
\end{bmatrix}e^{\begin{bmatrix}
0 & 0 \\
0 & -(u + v)t \\
\end{bmatrix}}\begin{bmatrix}
\frac{v}{u + v} & \frac{u}{u + v} \\
-\frac{1}{u + v} & \frac{1}{u + v} \\
\end{bmatrix} \\
&= \frac{1}{u + v}\begin{bmatrix}
1 & -u \\
1 & v \\
\end{bmatrix}\begin{bmatrix}
1 & 0 \\
0 & e^{-(u + v)t} \\
\end{bmatrix}\begin{bmatrix}
v & u \\
-1 & 1 \\
\end{bmatrix} \\
&= \frac{1}{u + v}\begin{bmatrix}
v + ue^{-(u + v)t} & u - ue^{-(u + v)t} \\
v - ve^{-(u + v)t} & u + ve^{-(u + v)t} 
\end{bmatrix}
\end{align*}
$$

As to the limiting distribution $\pi^{(t)}$, suppose that the system is
in state 1 at time $n = 0$ with probability ${\pi_{1}}^{(0)}$ and in
state 2 at time $n = 0$ with probability ${\pi_{2}}^{(0)}$, such that
$\pi^{(0)} = ({\pi_{1}}^{(0)},{\pi_{2}}^{(0)})$ and
${\pi_{1}}^{(0)} + {\pi_{2}}^{(0)} = 1$. It follows that

$$
\begin{align*}
\pi^{(t)} &= \pi^{(0)}P(t) \\
&= \frac{1}{u + v}\begin{bmatrix}
{\pi_{1}}^{(0)} & {\pi_{2}}^{(0)}
\end{bmatrix} \begin{bmatrix}
v + ue^{-(u + v)t} & u - ue^{-(u + v)t} \\
v - ve^{-(u + v)t} & u + ve^{-(u + v)t}
\end{bmatrix} \\
&= \frac{1}{u + v}\begin{bmatrix}
{\pi_{1}}^{(0)}(v + ue^{-(u + v)t}) + {\pi_{2}}^{(0)}(v + ue^{-(u + v)t}) \\
{\pi_{1}}^{(0)}(u - ue^{-(u + v)t}) + {\pi_{2}}^{(0)}(u + ve^{-(u + v)t})
\end{bmatrix}^{T}.
\end{align*}
$$

By letting $t \rightarrow \infty$,
$\lim_{t \rightarrow \infty}e^{-(u + v)t} = 0$. Hence, the limiting
distribution $\pi$ is given by

$$
\begin{align*}
\pi &= \lim_{t \rightarrow \infty} \pi^{(t)} = \begin{bmatrix}
\frac{v}{u + v} & \frac{u}{u + v}
\end{bmatrix}.
\end{align*}
$$

According to the text, in case $u=v=1$

$$
\begin{align*}
P(t) &= \frac{1}{2} \begin{bmatrix}
1 + e^{-2t} & 1 - e^{-2t} \\
1 - e^{-2t} & 1 + e^{-2t}
\end{bmatrix},
\end{align*}
$$

which is the binary equivalent of JC69.
