**Solution.**

(a) Set
    $\left( \log\left( f\left( x \middle| \theta \right) \right) \right)^{'}$
    to zero and solve the resulting equation:

$$
\begin{align*}
x(\log\theta)' + (n - x)(\log{(1 - \theta))}' &= 0 \\
\frac{x}{\theta} - \frac{(n - x)}{1 - \theta} &= 0 \\
\widehat{\theta} &= \frac{x}{n}.
\end{align*}
$$



(b) It is easy to see $\widehat{\theta} = \frac{x}{n}$ based on the result of (a) because the likelihood functions between (a) and (b) differ in only the constant term which contributes nothing to solving $\left( \log\left( f\left( x|\theta \right) \right) \right)^{'} = 0$.
