**Solution.**

According to Eq. (7.9) in (Yang 2014a), the transition probability is
defined as

$$p(x,y) = \left\{ \begin{array}{r}
q\left( y \middle| x \right) \bullet \alpha(x,y),y \neq x, \\
1 - \sum_{y \neq x}^{}{q\left( y \middle| x \right)\alpha(x,y),y = x,}
\end{array} \right.\ $$

where
$\alpha(x,y) = \min\left( 1,\frac{\pi(y)}{\pi(x)} \times \frac{q\left( x \middle| y \right)}{q\left( y \middle| x \right)} \right).$

a\)

Consider the symmetrical move, where by definition
$\( q(\bullet | \bullet) = \frac{1}{2} \).$
As given in the problem, $\pi_{1} \geq \pi_{2} \geq \pi_{3}$. Hence, the transition
matrix $P$ is given as

$$
{\alpha(1,2) = \frac{\pi_{2}}{\pi_{1}},
}{\alpha(1,3) = \frac{\pi_{3}}{\pi_{1}},
}{\alpha(2,1) = 1,
}{\alpha(2,3) = \frac{\pi_{3}}{\pi_{2}},
}{\alpha(3,1) = \alpha(3,2) = 1.}
$$

Accordingly,

$$
{P = \begin{bmatrix}
1 - \frac{\pi_{2}}{{2\pi}_{1}} - \frac{\pi_{3}}{{2\pi}_{1}} & \frac{\pi_{2}}{{2\pi}_{1}} & \frac{\pi_{3}}{{2\pi}_{1}} \\
\frac{1}{2} & 1 - \frac{1}{2} - \frac{\pi_{3}}{{2\pi}_{2}} & \frac{\pi_{3}}{{2\pi}_{2}} \\
\frac{1}{2} & \frac{1}{2} & 0
\end{bmatrix}
}{= \begin{bmatrix}
\frac{3}{2} - \frac{1}{{2\pi}_{1}} & \frac{\pi_{2}}{{2\pi}_{1}} & \frac{\pi_{3}}{{2\pi}_{1}} \\
\frac{1}{2} & \frac{1}{2} - \frac{\pi_{3}}{{2\pi}_{2}} & \frac{\pi_{3}}{{2\pi}_{2}} \\
\frac{1}{2} & \frac{1}{2} & 0
\end{bmatrix}.}
$$

b\)

Consider the asymmetrical move where
$q\left( 3 \middle| 1 \right) = q\left( 1 \middle| 2 \right) = q\left( 2 \middle| 3 \right) = \frac{2}{3}$
and
$q\left( 2 \middle| 1 \right) = q\left( 3 \middle| 2 \right) = q\left( 1 \middle| 3 \right) = \frac{1}{3}$.*\
*$${\alpha(1,2) = \min\left( 1,\frac{2\pi_{2}}{\pi_{1}} \right),
}{\alpha(1,3) = \min{\left( 1,\frac{\pi_{3}}{{2\pi}_{1}} \right) = \frac{\pi_{3}}{{2\pi}_{1}}},
}{\alpha(2,1) = \min\left( 1,\frac{\pi_{1}}{{2\pi}_{2}} \right),
}{\alpha(2,3) = \min\left( 1,\frac{2\pi_{3}}{\pi_{2}} \right),
}{\alpha(3,1) = \min\left( 1,\frac{2\pi_{1}}{\pi_{3}} \right) = 1,
}{\alpha(3,2) = \min\left( 1,\frac{\pi_{2}}{{2\pi}_{3}} \right).}$$

Consequently, we can derive the transition matrix $P$ as

$$P = \begin{bmatrix}
1 - \frac{1}{3}\min\left( 1,\frac{2\pi_{2}}{\pi_{1}} \right) - \frac{\pi_{3}}{{3\pi}_{1}} & \frac{1}{3}\min\left( 1,\frac{2\pi_{2}}{\pi_{1}} \right) & \frac{\pi_{3}}{{3\pi}_{1}} \\
{\frac{2}{3}\min}\left( 1,\frac{\pi_{1}}{{2\pi}_{2}} \right) & 1 - {\frac{2}{3}\min}\left( 1,\frac{\pi_{1}}{{2\pi}_{2}} \right) - \frac{1}{3}\min\left( 1,\frac{2\pi_{3}}{\pi_{2}} \right) & \frac{1}{3}\min\left( 1,\frac{2\pi_{3}}{\pi_{2}} \right) \\
\frac{1}{3} & \frac{2}{3}\min\left( 1,\frac{\pi_{2}}{{2\pi}_{3}} \right) & \frac{2}{3} - \frac{2}{3}\min\left( 1,\frac{\pi_{2}}{{2\pi}_{3}} \right)
\end{bmatrix}.$$
