**Solution.**

In Eq. (1.79) of (Yang 2014a), the transition probability matrix is
given as

$$P(t) = \ \begin{bmatrix}
p_{0} & p_{1} \\
p_{1} & p_{0}
\end{bmatrix},$$

where $p_{0} = \frac{1}{2} + \frac{1}{2}e^{- 2t}$ and
$p_{1} = \frac{1}{2} - \frac{1}{2}e^{- 2t}$.

Denote the state at node $i$ (either tip or ancestral node) as $S_{i}$.
According to the problem statement, $S_{i}$ are restricted to only two
values, which we assign as A or B. The following can be easily
calculated based on Section 4.2 of (Yang 2014a). Further, define
$a = e^{- 2t_{10}}$ and $b = e^{- 2t_{11}}$, thus
$e^{- 2\left( t_{10} + t_{11} \right)} = ab$.

Hence,

$${P(xxx) = P\left( S_{1} = A,S_{2} = A,S_{3} = A \right) + P\left( S_{1} = B,S_{2} = B,S_{3} = B \right)
}{= 2 \times P\left( S_{1} = A,S_{2} = A,S_{3} = A \right)
}{= 2 \times 0.5 \times \left( P\left( S_{1} = A,S_{2} = A,S_{3} = A \middle| S_{0} = A \right) + P\left( S_{1} = A,S_{2} = A,S_{3} = A \middle| S_{0} = B \right) \right)
}{= P\left( S_{1} = A,S_{2} = A,S_{3} = A,S_{4} = A \middle| S_{0} = A \right) + P\left( S_{1} = A,S_{2} = A,S_{3} = A,S_{4} = B \middle| S_{0} = A \right) + P\left( S_{1} = A,S_{2} = A,S_{3} = A,S_{4} = A \middle| S_{0} = B \right) + P\left( S_{1} = A,S_{2} = A,S_{3} = A,S_{4} = B \middle| S_{0} = B \right)
}{= \left( \frac{1}{2} + \frac{1}{2}e^{- 2\left( t_{10} + t_{11} \right)} \right)\left( \frac{1}{2} + \frac{1}{2}e^{- 2t_{10}} \right)\left( \frac{1}{2} + \frac{1}{2}e^{- 2t_{11}} \right)^{2} + \left( \frac{1}{2} + \frac{1}{2}e^{- 2\left( t_{10} + t_{11} \right)} \right)\left( \frac{1}{2} - \frac{1}{2}e^{- 2t_{10}} \right)\left( \frac{1}{2} - \frac{1}{2}e^{- 2t_{11}} \right)^{2} + \left( \frac{1}{2} - \frac{1}{2}e^{- 2\left( t_{10} + t_{11} \right)} \right)\left( \frac{1}{2} - \frac{1}{2}e^{- 2t_{10}} \right)\left( \frac{1}{2} + \frac{1}{2}e^{- 2t_{11}} \right)^{2} + \left( \frac{1}{2} - \frac{1}{2}e^{- 2\left( t_{10} + t_{11} \right)} \right)\left( \frac{1}{2} + \frac{1}{2}e^{- 2t_{10}} \right)\left( \frac{1}{2} - \frac{1}{2}e^{- 2t_{11}} \right)^{2}
}{= \frac{1}{16}\left( (1\  + \ ab)(1\  + \ a)(1\  + \ b)(1\  + \ b) + \ (1\  + \ ab)(1\  + \ a)(1\  - \ b)(1\  - \ b) + \ (1\  - \ ab)(1\  - \ a)(1\  + \ b)(1\  + \ b) + \ (1\  - \ ab)(1\  + \ a)(1\  - \ b)(1\  - \ b) \right)
}{= \frac{1}{16}\left( 4 + 2a - 4ab + 2a^{2}b + 4b^{2} + 2ab^{2} + a^{2}b^{2} + 2a^{2}b^{3} \right),}$$

$${P(xxy) = P\left( S_{1} = A,S_{2} = A,S_{3} = B \right) + P\left( S_{1} = B,S_{2} = B,S_{3} = A \right)
}{= 2 \times P\left( S_{1} = A,S_{2} = A,S_{3} = B \right)
}{= P\left( S_{1} = A,S_{2} = A,S_{3} = B,S_{4} = A \middle| S_{0} = A \right) + P\left( S_{1} = A,S_{2} = A,S_{3} = B,S_{4} = B \middle| S_{0} = A \right) + P\left( S_{1} = A,S_{2} = A,S_{3} = B,S_{4} = A \middle| S_{0} = B \right) + P\left( S_{1} = A,S_{2} = A,S_{3} = B,S_{4} = B \middle| S_{0} = B \right)
}{= \left( \frac{1}{2} - \frac{1}{2}e^{- 2\left( t_{10} + t_{11} \right)} \right)\left( \frac{1}{2} + \frac{1}{2}e^{- 2t_{10}} \right)\left( \frac{1}{2} + \frac{1}{2}e^{- 2t_{11}} \right)^{2} + \left( \frac{1}{2} - \frac{1}{2}e^{- 2\left( t_{10} + t_{11} \right)} \right)\left( \frac{1}{2} - \frac{1}{2}e^{- 2t_{10}} \right)\left( \frac{1}{2} - \frac{1}{2}e^{- 2t_{11}} \right)^{2} + \left( \frac{1}{2} + \frac{1}{2}e^{- 2\left( t_{10} + t_{11} \right)} \right)\left( \frac{1}{2} - \frac{1}{2}e^{- 2t_{10}} \right)\left( \frac{1}{2} + \frac{1}{2}e^{- 2t_{11}} \right)^{2} + \left( \frac{1}{2} + \frac{1}{2}e^{- 2\left( t_{10} + t_{11} \right)} \right)\left( \frac{1}{2} + \frac{1}{2}e^{- 2t_{10}} \right)\left( \frac{1}{2} - \frac{1}{2}e^{- 2t_{11}} \right)^{2}
}{= \frac{1}{16}\left\lbrack (1 - ab)(1 + a)(1 + b)(1 + b) + (1 - ab)(1 - a)(1 - b)(1 - b) + (1 + ab)(1 - a)(1 + b)(1 + b) + (1 + ab)(1 + a)(1 - b)(1 - b) \right\rbrack
}{= - \frac{1}{2}a^{2}b^{2} + \frac{1}{4}\left( b^{2} + 1 \right),}$$

$${P(yxx) = \ P\left( S_{1} = A,S_{2} = B,S_{3} = B \right) + P\left( S_{1} = B,S_{2} = A,S_{3} = A \right)
}{= 2 \times P\left( S_{1} = A,S_{2} = B,S_{3} = B \right)
}{= P\left( S_{1} = A,S_{2} = B,S_{3} = B,S_{4} = A \middle| S_{0} = A \right) + P\left( S_{1} = A,S_{2} = B,S_{3} = B,S_{4} = B \middle| S_{0} = A \right) + P\left( S_{1} = A,S_{2} = B,S_{3} = B,S_{4} = A \middle| S_{0} = B \right) + P\left( S_{1} = A,S_{2} = B,S_{3} = B,S_{4} = B \middle| S_{0} = B \right)
}{= \left( \frac{1}{2} - \frac{1}{2}e^{- 2\left( t_{10} + t_{11} \right)} \right)\left( \frac{1}{2} + \frac{1}{2}e^{- 2t_{10}} \right)\left( \frac{1}{2} + \frac{1}{2}e^{- 2t_{11}} \right)\left( \frac{1}{2} - \frac{1}{2}e^{- 2t_{11}} \right) + \left( \frac{1}{2} - \frac{1}{2}e^{- 2\left( t_{10} + t_{11} \right)} \right)\left( \frac{1}{2} - \frac{1}{2}e^{- 2t_{10}} \right)\left( \frac{1}{2} + \frac{1}{2}e^{- 2t_{11}} \right)\left( \frac{1}{2} - \frac{1}{2}e^{- 2t_{11}} \right) + \left( \frac{1}{2} + \frac{1}{2}e^{- 2\left( t_{10} + t_{11} \right)} \right)\left( \frac{1}{2} - \frac{1}{2}e^{- 2t_{10}} \right)\left( \frac{1}{2} + \frac{1}{2}e^{- 2t_{11}} \right)\left( \frac{1}{2} - \frac{1}{2}e^{- 2t_{11}} \right) + \left( \frac{1}{2} + \frac{1}{2}e^{- 2\left( t_{10} + t_{11} \right)} \right)\left( \frac{1}{2} + \frac{1}{2}e^{- 2t_{10}} \right)\left( \frac{1}{2} - \frac{1}{2}e^{- 2t_{11}} \right)^{2}
}{= \frac{1}{16}\left( (1 - ab)(1 + a)(1 + b)(1 - b) + (1 - ab)(1 - a)(1 + b)(1 - b) + (1 + ab)(1 - a)(1 + b)(1 - b) + (1 + ab)(1 + a)(1 - b)(1 - b) \right)
}{= \frac{1}{8}\left( a^{2}b^{3} - a^{2}b^{2} + \left( ab^{3} - ab \right) + \left( 2 - \left( b + b^{2} \right) \right) \right).}$$
