**Solution.**

\(a\) Refer to Eq. (2.10) in (Yang, 2006):

$$d_{S} = \frac{L_{2}A_{2} + L_{4}d_{4}}{\frac{L_{2}}{3} + L_{4}},\ d_{N} = \frac{L_{2}B_{2} + L_{0}d_{0}}{\frac{2}{3}L_{2} + L_{0}}.$$

According to the given information, we have $\alpha = \kappa\beta$,
$A_{0} = \alpha t\omega$, $B_{0} = 2\beta t\omega$, $A_{2} = \alpha t$,
$B_{2} = 2\beta t\omega$, $A_{4} = \alpha t$,
$B_{4} = 2\beta t$,$\ L_{0} = 2$, $L2 = 1 - \gamma$, and
$L_{4} = \gamma$. Hence,

$${d_{0} = A_{0} + B_{0} = \alpha t\omega + 2\beta t\omega},$$

$${d_{4} = A_{4} + B_{4} = \alpha t + 2\beta t.}$$

Plugging the above into Eq. (2.10) in (Yang, 2006), we have

$$
\begin{align*}
d_{S} &= \frac{(1 - \gamma)\alpha t + \gamma(\alpha t + 2\beta t)}{\frac{1 - \gamma}{3} + \gamma} \\
&= 3 \times \frac{(1 - \gamma)\kappa\beta t + \gamma(\kappa\beta t + 2\beta t)}{1 + 2\gamma} \\
&= \frac{3(\kappa + 2\gamma)\beta t}{1 - 2\gamma},
\end{align*}
$$

and

$$
\begin{align*}
d_{N} &= \frac{2\beta t\omega(1 - \gamma) + 2(\alpha t\omega + 2\beta t\omega)}{\frac{2}{3}(1 - \gamma) + 2} \\
&= \frac{3\left( \beta t\omega(1 - \gamma) + (\kappa\beta t\omega + 2\beta t\omega) \right)}{4 - \gamma} \\
&= \frac{3(\kappa + 3 - \gamma)\beta t\omega}{4 - \gamma}.
\end{align*}
$$

\(b\) As to LPB93, following Eq. (2.11) in (Yang, 2006), we have

$${d_{S} = \frac{L_{2}A_{2} + L_{4}A_{4}}{L_{2} + L_{4}} + B_{4}
}{= \frac{(1 - \gamma)\alpha t + \gamma\alpha t}{(1 - \gamma) + \gamma} + 2\beta t
}{= \alpha t + 2\beta t,}$$

$${d_{N} = A_{0} + \frac{L_{0}B_{0} + L_{2}B_{2}}{L_{0} + L_{2}}
}{= \alpha t\omega + \frac{2(2\beta t\omega) + (1 - \gamma) \times 2\beta t\omega}{2 + 1 - \gamma}
}{= \omega(\alpha t + 2\beta t).
}$$

As to LWL85m, we follow Eq. (2.12) in (Yang, 2006) to calculate $d_{S}$
as

$$
\begin{align*}
d_{S} &= \frac{L_{2}A_{2} + L_{4}d_{4}}{\rho L_{2} + L_{4}} \\
&= \frac{(1 - \gamma)\alpha t + \gamma(\alpha t + 2\beta t)}{\frac{\alpha t}{\alpha t + 2\beta t}(1 - \gamma) + \gamma} \\
&= \frac{(\alpha t + 2\beta t)(\alpha t + 2\gamma\beta t)}{\alpha t(1 - \gamma) + (\alpha t + 2\beta t)\gamma} \\
&= \alpha t + 2\beta t,
\end{align*}
$$

and $d_{N}$ as

$$
\begin{align*}
d_{N} &= \frac{L_{2}B_{2} + L_{0}d_{0}}{(1 - \rho)L_{2} + L_{0}} \\
&= \frac{(1 - \gamma)2\omega\beta t + 2(\omega\alpha t + 2\omega\beta t)}{\left( 1 - \frac{\alpha t}{\alpha t + 2\beta t} \right)(1 - \gamma) + 2} \\
&= \omega(\alpha t + 2\beta t)\frac{(1 - \gamma)\beta t + (\alpha t + 2\beta t)}{(1 - \gamma)\beta t + (\alpha t + 2\beta t)} \\
&= \ \omega d_{S}.
\end{align*}
$$


Note that in the above $\rho$ is given as
$\rho = \frac{A_{4}}{A_{4} + B_{4}}$ according to Eq (2.13) in (Yang,
2006).
